Renaming [SExpRec_pointer] to [SEXP] to be closer to the C.

low/debugType.ml
@@ -9,11 +9,11 @@ type funtype =
   | Result_int_list of (globals -> runs_type -> state -> int list result)
   | Result_float of (globals -> runs_type -> state -> float result)
   | Result_string of (globals -> runs_type -> state -> char list result)
-  | Result_pointer of (globals -> runs_type -> state -> sExpRec_pointer result)
+  | Result_pointer of (globals -> runs_type -> state -> sEXP result)
 
   | Argument_unit of (unit -> funtype)
   | Argument_bool of (bool -> funtype)
   | Argument_int of (int -> funtype)
   | Argument_float of (float -> funtype)
-  | Argument_pointer of (sExpRec_pointer -> funtype)
+  | Argument_pointer of (sEXP -> funtype)
 
